% chapter 8
\chapter{Jun 2014}
\shabox{Q5}\\
Given 
\begin{align*}
u_{rr}+\frac{1}{r}u-r+\frac{1}{r^2}u-{\theta\theta}&=0,\,r>c,\,\,-\pi\le\theta\le\pi\\
u(c,\theta)&=f(\theta),\,-\pi\le\theta\le\pi
\end{align*}
a) Determine the solutions for $R(r)$-problem:\\
Let $R=r^m,\,R^{'}=mr^{m-1},\,R^{''}=m(m-1)r^{m-2}$ and sunstitute into
\begin{align}
r^2R^{''}+rR^{'}-\lambda R&=0\\
r^2m(m-1)r^{m-2}+rmr^{m-1}-\lambda r^m&=0\\
(m^2-\lambda)r^m&=0\\
\text{Since $r^m\neq 0$},&\\
m&=0,0\leftarrow\shabox{for $\lambda=0$}\\
m&=n,-n\leftarrow\shabox{for $\lambda=n^2$}
\end{align}
The solution are
\begin{align}
R(r)&=c_1+c_2\,\ln\,r\label{q5j14a}\\
R(r)&=c_1r^n+c_2r^{-n}\label{q5j14b}
\end{align}
$R(r)$ are unbounded as $r$ approaches to $\infty$.\\
The solution of $R(r)$-problem are
\begin{align}
R(r)&=c_1\\
R(r)&=c_2r^{-n}
\end{align}


b)Thus The product  solution is
\begin{align}
u_n(r,\theta)&=A_0c_1+c_2r^{-n}(c_1\,\cos\,n\theta+c_2\,\sin\,n\theta)\\
&=B_0+r^{-n}(A_n\,\cos\,n\theta+B_n\,\sin\,n\theta)\leftarrow\shabox{$B_0=A_0c_1$, $A_n=c_1c_2$, $B_n=c_1c_2$}
\end{align}
Hence the general solution is
\begin{align}
u(r,\theta)&=B_0+\sum_{n=1}^\infty\,r^{-n}(A_n\,\cos\,n\theta+B_n\,\sin\,n\theta)\label{soq5j14}
\end{align}
Now apply BC:$f(\theta)=u(1,\theta)=\pi-|\theta|$
\begin{align*}
B_0&=\frac{1}{2\pi}\int_{-\pi}^{\pi}(\pi-|\theta|)\,d\theta\\
&=\frac{1}{2\pi}\int_{-\pi}^0(\pi-(-\theta))\,d\theta+\frac{1}{2\pi}\int_{0}^{\pi}(\pi-\theta)\,d\theta\\
&=\frac{1}{2\pi}\left[\pi\theta+\frac{1}{2}\theta^2\right]_{-\pi}^0+\frac{1}{2\pi}\left[\pi\theta-\frac{1}{2}\theta^2\right]_0^\pi\\
&=\frac{1}{2\pi}(0-(\pi^2+\frac{1}{2}\pi^2)+\frac{1}{2\pi}(\pi^2-\frac{1}{2}\pi^2)\\
&=\frac{1}{2}\pi
\end{align*}
\begin{align*}
A_n&=\frac{1}{\pi}\int_{-\pi}^\pi(\pi-|\theta|)\,\cos\,n\theta\,d\theta\\
&=\frac{1}{\pi}\int_{-\pi}^0(\pi+\theta)\cos\,n\theta\,d\theta+\frac{1}{\pi}\int_0^\pi(\pi-\theta)\cos\,n\pi\,d\theta\\
&=-\frac{(-1+(-1)^2)}{\pi n^2}+-\frac{(-1+(-1)^2)}{\pi n^2}\\
&=-\frac{2(-1+(-1)^n)}{\pi n^2}
\end{align*}
\begin{align}
B_n&=\frac{1}{\pi}\int_{-\pi}^\pi(\pi-|\theta|)\,\sin\,n\theta\,d\theta\nonumber\\
&=\frac{1}{\pi}\int_{-\pi}^0(\pi+\theta)\sin\,n\theta\,d\theta+\frac{1}{\pi}\int_0^\pi(\pi-\theta)\sin\,n\theta\,d\theta\nonumber\\
&=\frac{(-\pi n+\sin(\pi n))}{\pi n^2}-\frac{(-\pi n+\sin(\pi n))}{\pi n^2}\\
&=0
\end{align}
The solution is give by \eqref{soq5j14} where $B_0$, $A_n$ and $B_n$ is given by the above .



